WIP - new WF properties on the DCFG

examples/Imp2Vir/CFGC_Interface.v
@@ -44,21 +44,27 @@ Section FreshnessMonad.
 
   Definition wf_outputs (g : dcfg) : Prop :=
     snd (outs g) = List.length (fst (outs g))
-    /\ List.incl (fst (outs g)) (outputs (graph g)).
+    /\ List.incl (fst (outs g)) (outputs (graph g))
+    /\ Coqlib.list_disjoint (fst (outs g)) (inputs (graph g)) .
+
+  Definition wf_graph (g : dcfg) : Prop :=
+    wf_ocfg_bid (graph g).
 
   Definition wf_dcfg (g : dcfg) : Prop :=
     wf_inputs g
-    /\ wf_outputs g.
+    /\ wf_outputs g
+    /\ wf_graph g .
   
   Definition empty_dcfg : dcfg := (mk_dcfg [] [] []).
 
   Lemma empty_wf : wf_dcfg empty_dcfg.
   Proof.
-    unfold empty_dcfg, wf_dcfg, wf_inputs, wf_outputs.
-    intuition.
+    unfold empty_dcfg, wf_dcfg, wf_inputs, wf_outputs, wf_graph, wf_ocfg_bid.
+    intuition ; simpl.
+    apply Util.list_disjoint_nil_r.
+    apply Coqlib.list_norepet_nil.
   Qed.
 
-  (* Could be a fresh/state monad *)
   Record FST :=
     mk_FST
       {
@@ -153,168 +159,6 @@ End InterfaceCombinators.
 
 From Vellvm Require Import Utils.Tactics.
 
-Lemma wf_mk_block : forall σ c, wf_dcfg (snd ((mk_block c) σ )).
-Proof.
-  intros.
-  unfold wf_dcfg, wf_inputs, wf_outputs, mk_block.
-  destruct σ ; cbn.
-  unfold incl.
-  intuition
-  ; try reflexivity
-  ; try (cbn in * ; assumption).
-Qed.
-
-Lemma wf_mk_seq : forall σ g1 g2 out1 in2,
-    wf_dcfg g1 -> (* recursive use of the interface *)
-    wf_dcfg g2 ->
-    wf_dcfg (snd ((mk_seq g1 g2 out1 in2) σ )).
-Proof.
-  intros *  WF_G1 WF_G2.
-  unfold wf_dcfg, wf_inputs, wf_outputs, mk_seq.
-  destruct σ ; cbn.
-  unfold wf_dcfg, wf_inputs, wf_outputs in WF_G1, WF_G2.
-  destruct WF_G1 as [[LEN_INS_G1 INPUTS_G1] [LEN_OUT_G1 OUTPUTS_G1]].
-  destruct WF_G2 as [[LEN_INS_G2 INPUTS_G2] [LEN_OUT_G2 OUTPUTS_G2]].
-  unfold incl in *.
-  simpl in *.
-  intuition ;
-    repeat flatten_all.
-  - inv Heq0. reflexivity.
-  - unfold cfg_seq.
-    simpl in *.
-    rewrite Util.list_cons_app ;
-    rewrite !CFGC_Utils.inputs_app in *.
-    apply in_app_or in H.
-    apply in_or_app.
-    destruct H as [ H | H ].
-    + left. now apply INPUTS_G1.
-    + right ; apply in_or_app ; right.
-      apply INPUTS_G2.
-      rewrite remove_ListRemove in H ;
-      apply in_remove in H. intuition.
-  - inv Heq0. reflexivity.
-  - unfold cfg_seq.
-    simpl in *.
-    rewrite Util.list_cons_app ;
-    rewrite !ScopeTheory.outputs_app in *.
-    apply in_app_or in H.
-    apply in_or_app.
-    destruct H as [ H | H ].
-    + left. apply OUTPUTS_G1.
-      rewrite remove_ListRemove in H ;
-      apply in_remove in H. intuition.
-    + right ; apply in_or_app ; right.
-      now apply OUTPUTS_G2.
-Qed.
-
-Lemma wf_mk_join : forall σ g out1 out2,
-    wf_dcfg g ->
-    wf_dcfg (snd ((mk_join g out1 out2) σ)).
-Proof.
-  intros * WF_G.
-  unfold wf_dcfg, wf_inputs, wf_outputs, mk_seq.
-  destruct σ ; cbn.
-  unfold wf_dcfg, wf_inputs, wf_outputs in WF_G.
-  destruct WF_G as [[LEN_INS_G INPUTS_G] [LEN_OUT_G OUTPUTS_G]].
-  unfold incl in *.
-  repeat flatten_all.
-  simpl in *.
-  intuition.
-  - inv Heq0.
-    apply INPUTS_G in H.
-    unfold cfg_join.
-    rewrite Util.list_cons_app ;
-    rewrite !CFGC_Utils.inputs_app in *.
-    apply in_or_app. now left.
-  - rewrite H0.
-    unfold cfg_join.
-    rewrite Util.list_cons_app ;
-    rewrite !ScopeTheory.outputs_app in *.
-    apply in_or_app ; right. 
-    apply in_or_app ; right. simpl ; intuition.
-  - unfold cfg_join.
-    rewrite Util.list_cons_app
-    ; rewrite !ScopeTheory.outputs_app in *.
-    inv Heq1 ; clear H.
-    apply in_or_app ; left.
-    apply OUTPUTS_G.
-    rewrite remove_ListRemove in H0 ;
-      apply in_remove in H0 ; destruct H0 as [H0 _].
-    rewrite remove_ListRemove in H0 ;
-      apply in_remove in H0 ; destruct H0 as [H0 _].
-    assumption.
-Qed.
-    
-Lemma wf_mk_branch : forall σ cond gT gF inT inF,
-    wf_dcfg gT ->
-    wf_dcfg gF ->
-    wf_dcfg (snd ((mk_branch cond gT gF inT inF) σ)).
-Proof.
-  intros *  WF_GT WF_GF.
-  unfold wf_dcfg, wf_inputs, wf_outputs, mk_seq.
-  destruct σ ; cbn.
-  unfold wf_dcfg, wf_inputs, wf_outputs in WF_GT, WF_GF.
-  destruct WF_GT as [[LEN_INS_GT INPUTS_GT] [LEN_OUT_GT OUTPUTS_GT]].
-  destruct WF_GF as [[LEN_INS_GF INPUTS_GF] [LEN_OUT_GF OUTPUTS_GF]].
-  unfold incl in *.
-  simpl in *.
-  intuition ;
-    repeat flatten_all ; simpl in * ; try auto.
-  - intuition. right.
-    inv Heq0.
-    rewrite !ScopeTheory.inputs_app.
-    apply in_or_app.
-    apply in_app_or in H0.
-    destruct H0 ; [left ; apply INPUTS_GT | right ; apply INPUTS_GF] ;
-    now rewrite remove_ListRemove in H0
-    ; apply in_remove in H0
-    ; destruct H0 as [H0 _].
-  - inv Heq1. clear H0.
-    rewrite Util.list_cons_app
-    ; rewrite !ScopeTheory.outputs_app in *.
-    apply in_or_app ; right.
-    apply in_or_app.
-    apply in_app_or in H.
-    destruct H ; [left ; apply OUTPUTS_GT | right ; apply OUTPUTS_GF] ; assumption.
-Qed.
-
-Lemma wf_mk_while : forall σ expr_code cond gB inB outB,
-    wf_dcfg gB ->
-    wf_dcfg (snd ((mk_while expr_code cond gB inB outB) σ)).
-Proof.
-  intros * WF_G.
-  unfold wf_dcfg, wf_inputs, wf_outputs, mk_seq.
-  destruct σ ; cbn.
-  unfold wf_dcfg, wf_inputs, wf_outputs in WF_G.
-  destruct WF_G as [[LEN_INS_G INPUTS_G] [LEN_OUT_G OUTPUTS_G]].
-  unfold incl in *.
-  repeat flatten_all.
-  simpl in *.
-  intuition.
-  - inv Heq0.
-    right.
-    rewrite !ScopeTheory.inputs_app.
-    apply in_or_app ; left.
-    apply INPUTS_G.
-    now rewrite remove_ListRemove in H0
-    ; apply in_remove in H0.
-  - rewrite H0.
-    clear.
-    rewrite Util.list_cons_app
-    ; rewrite !ScopeTheory.outputs_app in *.
-    apply in_or_app ; left ; cbn ; intuition.
-  - inv Heq1.
-    rewrite Util.list_cons_app
-    ; rewrite !ScopeTheory.outputs_app in *.
-    apply in_or_app ; right.
-    apply in_or_app ; left.
-    apply OUTPUTS_G.
-    now rewrite remove_ListRemove in H0
-    ; apply in_remove in H0.
-Qed.
-
-
-From Coq Require Import Lia.
 Lemma neq_name : forall n1 n2, name n1 <> name n2 <-> n1 <> n2.
 Proof.
   intros.
@@ -329,6 +173,294 @@ Proof.
     rewrite H1 in H .
     contradiction.
 Qed.
+
+From Coq Require Import Lia.
+Lemma wf_mk_block : forall σ c, wf_dcfg (snd ((mk_block c) σ )).
+Proof.
+  intros.
+  unfold wf_dcfg, wf_inputs, wf_outputs, mk_block, wf_graph, wf_ocfg_bid.
+  destruct σ ; cbn.
+  unfold incl.
+  intuition
+  ; try reflexivity
+  ; try (cbn in * ; assumption)
+  ; try apply List_norepet_singleton.
+  apply Util.list_disjoint_singletons.
+  rewrite neq_name. lia.
+Qed.
+
+Ltac break_list_hyp :=
+  match goal with
+    | h: List.In _ (_ ++ _) |- _ => repeat (apply in_app_or in h)
+  end.
+
+Ltac break_list_goal :=
+  try (rewrite Util.list_cons_app) ;
+  try (
+  match goal with
+  | |- context[inputs (_ ++ _)] =>
+      repeat (rewrite !ScopeTheory.inputs_app)
+  | |- context[outputs (_ ++ _)] =>
+      repeat (rewrite !ScopeTheory.outputs_app)
+  end ) ;
+  try (
+  match goal with
+  | |- context[List.In _ (_ ++ _)] => repeat (apply in_or_app)
+  end).
+
+Lemma in_remove : forall l x y, List.In x (remove y l) -> List.In x l.
+Proof. intros.
+       rewrite remove_ListRemove in H
+       ; apply in_remove in H.
+       intuition.
+Qed.
+
+Ltac in_list :=
+  match goal with
+  | h: List.In _ _  |- _ => apply in_remove in h
+  end.
+
+Lemma wf_mk_seq : forall σ g1 g2 out1 in2,
+    wf_dcfg g1 -> (* recursive use of the interface *)
+    wf_dcfg g2 ->
+    wf_dcfg (snd ((mk_seq g1 g2 out1 in2) σ )).
+Proof.
+  intros *  WF_G1 WF_G2.
+  unfold wf_dcfg, wf_inputs, wf_outputs, mk_seq, wf_graph, wf_ocfg_bid.
+  destruct σ ; cbn.
+  unfold wf_dcfg, wf_inputs, wf_outputs, wf_graph, wf_ocfg_bid in WF_G1, WF_G2.
+  destruct WF_G1 as [[LEN_INS_G1 INPUTS_G1]
+                       [[LEN_OUT_G1 [OUTPUTS_G1 DISJOINTS_G1]] WF_BID_G1]].
+  destruct WF_G2 as [[LEN_INS_G2 INPUTS_G2]
+                       [[LEN_OUT_G2 [OUTPUTS_G2 DISJOINTS_G2]] WF_BID_G2]].
+  unfold incl in *.
+  simpl in *.
+  intuition ;
+    repeat flatten_all.
+  - inv Heq0. reflexivity.
+  - unfold cfg_seq.
+    simpl in *.
+    break_list_goal.
+    break_list_hyp.
+    match goal with
+    | h: List.In _ _ \/ List.In _ _ |- _ => destruct h
+    end.
+    + left. now apply INPUTS_G1.
+    + right ; right.
+      apply INPUTS_G2.
+      now in_list.
+  - inv Heq0. reflexivity.
+  - unfold cfg_seq.
+    simpl in *.
+    break_list_goal.
+    break_list_hyp.
+    match goal with
+    | h: List.In _ _ \/ List.In _ _ |- _ => destruct h
+    end.
+    + left. apply OUTPUTS_G1.
+      now in_list.
+    + right ; apply in_or_app ; right.
+      now apply OUTPUTS_G2.
+  - unfold cfg_seq.
+    simpl in *.
+    break_list_goal.
+    (* NOTE i'm stuck here, because I can't say anything about
+       for instance, the disjointness between l2 and (input graph0)
+     *)
+    admit.
+  - unfold cfg_seq.
+    simpl in *.
+    break_list_goal.
+    simpl.
+    apply Coqlib.list_norepet_append ; try assumption.
+    break_list_goal.
+    apply Coqlib.list_norepet_append ; try assumption.
+    apply List_norepet_singleton.
+    (* NOTE: Coqlib.list_disjoint [out1] (inputs G2) *)
+    (* a property I'd really like to have, via independent_flows, but how ? *)
+    admit.
+    apply Coqlib.list_disjoint_cons_r.
+    (* NOTE: Coqlib.list_disjoint (inputs G1) (inputs G2) *)
+    admit.
+    (* I need 2 things:
+       - new hypothesis (out1 ∈ (fst (outs dg)))
+          --> the programmer will have to prove that, but easy if he uses the
+              interface correctly
+       - new wf property on dcfg, st ∀ bk ∈ (fst (outs dg)), bk ∉ (graph dg)
+     *)
+    admit.
+Abort.
+
+Lemma wf_mk_join : forall σ g out1 out2,
+    wf_dcfg g ->
+    wf_dcfg (snd ((mk_join g out1 out2) σ)).
+Proof.
+  intros * WF_G.
+  unfold wf_dcfg, wf_inputs, wf_outputs, mk_seq, wf_graph, wf_ocfg_bid.
+  destruct σ ; cbn.
+  unfold wf_dcfg, wf_inputs, wf_outputs, wf_graph, wf_ocfg_bid in WF_G.
+  destruct WF_G as [[LEN_INS_G INPUTS_G]
+                       [[LEN_OUT_G [OUTPUTS_G DISJOINTS_G]] WF_BID_G]].
+  unfold incl in *.
+  repeat flatten_all.
+  simpl in *.
+  intuition.
+  - inv Heq0.
+    apply INPUTS_G in H.
+    unfold cfg_join.
+    break_list_goal.
+    now left.
+  - rewrite H0.
+    unfold cfg_join.
+    break_list_goal.
+    simpl ; intuition.
+  - unfold cfg_join.
+    break_list_goal.
+    inv Heq1 ; clear H.
+    left.
+    apply OUTPUTS_G.
+    repeat in_list.
+    assumption.
+  - unfold cfg_join.
+    break_list_goal.
+    simpl in *.
+    apply Coqlib.list_disjoint_cons_l.
+    (* I need lemmas about remove, but it should be easy here *)
+    admit.
+    (* freshness of (name counter_bid0)*)
+    admit.
+  - unfold cfg_join.
+    break_list_goal.
+    simpl in *.
+    apply Coqlib.list_norepet_append ; try assumption.
+    (* NOTE out1 ≠ out2 *)
+    (* ... should I need new wf property on outputs ? (no_repeat) *)
+    (* ... or hypothesis let to the programmer ? *)
+    admit.
+    (* NOTE Coqlib.list_disjoint (inputs graph0) [out1; out2] *)
+    (* I need 2 things:
+       - new hypothesis (out1, out2 ∈ (fst (outs dg)))
+          --> the programmer will have to prove that, but easy if he uses the
+              interface correctly
+       - new wf property on dcfg, st ∀ bk ∈ (fst (outs dg)), bk ∉ (graph dg)
+     *)
+    admit.
+Abort.
+    
+Lemma wf_mk_branch : forall σ cond gT gF inT inF,
+    wf_dcfg gT ->
+    wf_dcfg gF ->
+    wf_dcfg (snd ((mk_branch cond gT gF inT inF) σ)).
+Proof.
+  intros *  WF_GT WF_GF.
+
+  unfold wf_dcfg, wf_inputs, wf_outputs, mk_seq, wf_graph, wf_ocfg_bid.
+  destruct σ ; cbn.
+  unfold wf_dcfg, wf_inputs, wf_outputs, wf_graph, wf_ocfg_bid in WF_GT, WF_GF.
+  destruct WF_GT as [[LEN_INS_GT INPUTS_GT]
+                       [[LEN_OUT_GT [OUTPUTS_GT DISJOINTS_GT]] WF_BID_GT]].
+  destruct WF_GF as [[LEN_INS_GF INPUTS_GF]
+                       [[LEN_OUT_GF [OUTPUTS_GF DISJOINTS_GF]] WF_BID_GF]].
+  unfold incl in *.
+  simpl in *.
+  intuition ;
+    repeat flatten_all ; simpl in * ; try auto.
+  - intuition. right.
+    inv Heq0.
+    break_list_goal.
+    break_list_hyp.
+    match goal with
+    | h: List.In _ _ \/ List.In _ _ |- _ => destruct h
+    end
+    ; [left ; apply INPUTS_GT | right ; apply INPUTS_GF]
+    ; now in_list.
+  - inv Heq1 ; clear H0.
+    break_list_goal.
+    break_list_hyp.
+    right.
+    break_list_goal.
+    match goal with
+    | h: List.In _ _ \/ List.In _ _ |- _ => destruct h
+    end
+    ; [left ; apply OUTPUTS_GT | right ; apply OUTPUTS_GF]
+    ; assumption.
+  - apply Coqlib.list_disjoint_cons_r.
+    (* NOTE Coqlib.list_disjoint (l0 ++ l2) (inputs (graph0 ++ graph1)*)
+    admit.
+    (* freshness (name counter_bid0)*)
+    admit.
+  - break_list_goal.
+    apply Coqlib.list_norepet_append ; try assumption.
+    apply List_norepet_singleton.
+    apply Coqlib.list_norepet_append ; try assumption.
+    (* NOTE: Coqlib.list_disjoint (inputs GT) (inputs GF) *)
+    admit.
+    apply Util.list_disjoint_singleton_left.
+    (* freshness (name counter_bid0) *)
+    admit.
+Abort.
+
+Lemma wf_mk_while : forall σ expr_code cond gB inB outB,
+    wf_dcfg gB ->
+    wf_dcfg (snd ((mk_while expr_code cond gB inB outB) σ)).
+Proof.
+  intros * WF_G.
+  unfold wf_dcfg, wf_inputs, wf_outputs, mk_seq, wf_graph, wf_ocfg_bid.
+  destruct σ ; cbn.
+  unfold wf_dcfg, wf_inputs, wf_outputs, wf_graph, wf_ocfg_bid in WF_G.
+  destruct WF_G as [[LEN_INS_G INPUTS_G]
+                       [[LEN_OUT_G [OUTPUTS_G DISJOINTS_G]] WF_BID_G]].
+  unfold incl in *.
+  repeat flatten_all.
+  simpl in *.
+  intuition.
+  - inv Heq0.
+    right.
+    do 2 break_list_goal ; simpl.
+    left.
+    apply INPUTS_G.
+    now in_list.
+  - rewrite H0.
+    clear.
+    do 2 (break_list_goal ; simpl).
+    left ; cbn ; intuition.
+  - inv Heq1.
+    break_list_goal ; simpl.
+    right.
+    break_list_goal ; simpl.
+    left.
+    apply OUTPUTS_G.
+    now in_list.
+  - break_list_goal.
+    simpl in *.
+    apply Coqlib.list_disjoint_cons_l.
+    apply Coqlib.list_disjoint_cons_r.
+    (* lemma on remove - easy *)
+    admit.
+    (* freshness (name counter_bid0) *)
+    admit.
+    (* freshness (name counter_bid0) *)
+    admit.
+  - break_list_goal.
+    simpl in *.
+    break_list_goal.
+    apply Coqlib.list_norepet_append ; try assumption.
+    apply List_norepet_singleton.
+    apply Coqlib.list_norepet_append ; try assumption.
+    apply List_norepet_singleton.
+    apply Util.list_disjoint_singleton_right.
+    (* NOTE: ~ List.In outB (inputs gB)
+       - outB ∈ (outs gB)
+       - disjonction (inputs gB) (outs gB)
+     *)
+    admit.
+    apply Util.list_disjoint_singleton_left.
+    intro.
+    break_list_hyp.
+    (* NOTE: freshness (name counter_bid0) *)
+    admit.
+Abort.
+
 
 Lemma wf_mk_block_bind :
   forall σ0 σ1 σ2 c1 c2 g1 g2,
@@ -361,3 +493,32 @@ Proof.
     end ;
     now apply contra in H.
 Qed.
+
+(* NOTE: Now, I want a similar lemma, but with X states between
+         the 1st mk_block and the 2nd mk_block *)
+
+(* NOTE: Now, I want a similar lemma, but I can ALSO use other operations,
+         such mk_seq (instead of mk_block) *)
+
+(* Lemma wf_mk_seq_wf_seq : forall g1 g2 out1 in2, *)
+(*     List.In out1 (fst (outs g1)) -> (* easy to ensure *) *)
+(*     List.In in2 (fst (ins g2)) -> *)
+(*     wf_dcfg g1 -> (* recursive use of the interface *) *)
+(*     wf_dcfg g2 -> *)
+(*     wf_seq (graph g1) (graph g2) out1 in2. *)
+(* Proof. *)
+(*   intros * CORRECT_OUT1 CORRECT_IN2 WF_G1 WF_G2. *)
+(*   unfold wf_dcfg, wf_inputs, wf_outputs in WF_G1, WF_G2. *)
+(*   destruct WF_G1 as [[LEN_INS_G1 INPUTS_G1] [LEN_OUT_G1 OUTPUTS_G1]]. *)
+(*   destruct WF_G2 as [[LEN_INS_G2 INPUTS_G2] [LEN_OUT_G2 OUTPUTS_G2]]. *)
+(*   unfold wf_seq. *)
+
+(*
+In order to use the interface, the function compile should
+work with dcfg instead of ocfg.
+It remains some properties to prove, as
+`List.In out1 (fst (outs g1))`, but if the user uses the interface
+correctly, this is very easy to ensure.
+In this example, the user should pick out1 using the information
+in the DCFG (the outputs here).
+ *)
